Correctness.v
@@ -156,7 +156,7 @@ Proof.
     destruct argTcVal as [sttya [Weaka [TcHeapa TcVal_v']]]; eauto.
     
     inversion TcVal_cls as [ | | | 
-                             ? ? ? ? ? ? ? TcRho_rho' TcEnv_env' TcExp_abs [A B C D HSubst] 
+                             ? ? ? ? ? ? ? TcRho_rho' TcEnv_env' TcExp_abs ? [A B C D HSubst]  
                              | | |]; subst. 
     inversion TcExp_abs as [ | | | 
                              ? ? ? ? ? ? ? ? ? ? ? HBt_ec_ee TcExp_ec' TcExp_ee' 
@@ -265,7 +265,7 @@ Proof.
      destruct clsTcVal as [sttyb [Weakb [TcHeapb TcVal_cls]]]; eauto.
      
      inversion TcVal_cls as [ | | | 
-                              ? ? ? ? ? ? ? TcRho_rho' TcEnv_env' TcExp_abs [A B C D HSubst] 
+                              ? ? ? ? ? ? ? TcRho_rho' TcEnv_env' TcExp_abs ? [A B C D HSubst] 
                               | | |]; subst. 
      inversion TcExp_abs as [ | | | |
                               ? ? ? ? ? ?  HNo HLc1 HLc2 HBt_eb HTExp_eb
@@ -318,7 +318,7 @@ Proof.
     destruct argTcVal as [sttya [Weaka [TcHeapa TcVal_v']]]; eauto.
     
     inversion TcVal_cls as [ | | | 
-                             ? ? ? ? ? ? ? TcRho_rho' TcEnv_env' TcExp_abs [A B C D HSubst] 
+                             ? ? ? ? ? ? ? TcRho_rho' TcEnv_env' TcExp_abs ? [A B C D HSubst] 
                              | | |]; subst. 
     inversion TcExp_abs as [ | | | 
                              ? ? ? ? ? ? ? ? ? ? HBt_ec_ee TcExp_ec' TcExp_ee' 
