TypeSystem.v
@@ -465,10 +465,11 @@ Lemma ty_sound_closure:
   forall stty rgns env rho ctxt f x ec ee tyx tyc effc effe, 
     TcRho (rho, rgns) -> 
     TcEnv (stty, rho, env, ctxt) ->
-    TcExp (ctxt, rgns,  Mu f x ec ee, Ty2_Arrow tyx effc tyc effe Ty2_Effect, Empty_Static_Action) ->  
+    TcExp (ctxt, rgns,  Mu f x ec ee, Ty2_Arrow tyx effc tyc effe Ty2_Effect, Empty_Static_Action) -> 
+    (forall r : Name, r # subst_rho rho (Ty2_Arrow tyx effc tyc effe Ty2_Effect)) ->
     TcVal (stty, Cls (env, rho,  Mu f x ec ee),  subst_rho rho (Ty2_Arrow tyx effc tyc effe Ty2_Effect)).   
 Proof.
-  intros; econstructor; eassumption.
+  intros; econstructor; eauto.
 Qed.
 
 Lemma ty_sound_region_closure:
@@ -476,9 +477,11 @@ Lemma ty_sound_region_closure:
     TcRho (rho, rgns) -> 
     TcEnv (stty, rho, env,ctxt) ->
     TcExp (ctxt, rgns, Lambda x er, Ty2_ForallRgn (close_var_eff x effr) (close_var x tyr),  Empty_Static_Action) ->
+    (forall r : Name,
+       r # subst_rho rho (Ty2_ForallRgn (close_var_eff x effr) (close_var x tyr))) ->
     TcVal (stty, Cls (env, rho, Lambda x er), subst_rho rho (Ty2_ForallRgn (close_var_eff x effr) (close_var x tyr))).
 Proof.
-  intros. econstructor; eassumption.
+  intros. econstructor; eauto.
 Qed.  
   
 Lemma weakening_trans :
@@ -503,9 +506,19 @@ Proof.
   unfold not_set_elem in H2. unfold Ensembles.Complement in H2. 
   unfold not. intro. 
   apply RMapP.in_find_iff in H. 
-  apply H2. (* double negation *)
-  eapply H3; eassumption.
+  apply H2. 
+  eapply H0; eassumption.
 Qed.  
+
+Axiom subst_rho_close_var:
+  forall x rho tyr,
+     R.find (elt:=nat) x rho = None ->
+     (subst_rho rho (close_var x tyr) = (close_var x tyr)).
+
+Axiom subst_rho_close_var_eff :
+  forall x rho effr,
+    R.find (elt:=nat) x rho = None ->
+    fold_subst_eps rho (close_var_eff x effr) = (close_var_eff x effr).
 
 Lemma ty_sound:
   forall e env rho hp hp' v dynamic_eff,
@@ -535,18 +548,23 @@ Proof.
     eapply ty_sound_var; eassumption. 
   Case "mu_abs". 
     exists stty; (split; [| split]; auto).
-    eapply ty_sound_closure; try (solve [eassumption]).
+    eapply ty_sound_closure; try (solve [eassumption]); auto.
   Case "rgn_abs". 
     exists stty;  (split; [| split]; auto). 
-    eapply ty_sound_region_closure; try (solve [eassumption]).
+    eapply ty_sound_region_closure; try (solve [eassumption]). 
+    assert (R.find (elt:=nat) x rho = None) by 
+        (inversion Hrho; eapply contrapositiveTcRho; eauto).
+    rewrite subst_rho_forallrgn. 
+    rewrite subst_rho_close_var; auto. 
+    rewrite subst_rho_close_var_eff; auto. 
   Case "mu_app".   
     edestruct IHD1 as [sttym [Weak1 [TcHeap1 TcVal_mu]]]; eauto. 
     edestruct IHD2 as [sttya [Weaka [TcHeapa TcVal_arg]]]; eauto.  
     eapply ext_stores__env; eauto.  
     inversion TcVal_mu as [ | | | ? ? ? ? ? ? ?   TcRho_rho' TcEnv_env' TcExp_abs | | |] ; subst.      
     inversion TcExp_abs as [ | |  | ? ? ? ? ? ? ? ? ? ? ? ? TcExp_ec TcExp_ee | | | | | | | | | | | | | | | | | | | | | ]; subst. 
-    rewrite <- H4 in TcVal_mu. 
-    do 2 rewrite subst_rho_arrow in H4. inversion H4.
+    rewrite <- H5 in TcVal_mu. 
+    do 2 rewrite subst_rho_arrow in H5. inversion H5.
     assert (SubstEq1: subst_rho rho' tyx = subst_rho rho tya) by assumption. 
     assert (SubstEq2: subst_rho rho' tyc = subst_rho rho t) by assumption.
     rewrite <- SubstEq1 in TcVal_arg.
@@ -563,9 +581,9 @@ Proof.
     edestruct IHD2 as [sttyr [Weak2 [TcHeap2 TcVal_res]]]; eauto using update_env, ext_stores__env.
     apply update_rho. assumption. assumption. eapply extended_rho; eauto. 
     exists sttyr; intuition. 
-    rewrite subst_rho_forallrgn in H5.
-    rewrite subst_rho_forallrgn in H5.
-    inversion H5.  
+    rewrite subst_rho_forallrgn in H6.
+    rewrite subst_rho_forallrgn in H6.
+    inversion H6.  
     unfold update_R in TcVal_res. 
     simpl in TcVal_res. rewrite subst_add_comm in TcVal_res.
     SCase "abstraction body is well typed".
@@ -584,9 +602,9 @@ Proof.
       apply update_env.
       SSCase "TcEnv". apply update_env.
         SSSCase "Extended". eapply ext_stores__env; eauto.
-        SSSCase "Extended TcVal". rewrite <- H4 in TcVal_mu.  eapply ext_stores__val; eauto.
-      SSCase "TcVal". do 2 rewrite subst_rho_arrow in H4.
-          inversion H4.
+        SSSCase "Extended TcVal". rewrite <- H5 in TcVal_mu.  eapply ext_stores__val; eauto.
+      SSCase "TcVal". do 2 rewrite subst_rho_arrow in H5.
+          inversion H5.
           assert (SubstEq: subst_rho rho' tyx = subst_rho rho tya) by assumption.
           rewrite <- SubstEq in TcVal_arg.  eassumption. 
     exists sttyb. intuition.
@@ -603,6 +621,7 @@ Proof.
     SCase "TcHeap".
       eapply UnionTcHeap with (theta1:=theta1) (theta2:=theta2); eauto. 
     SCase "TcVal".
+      rewrite subst_rho_pair.
       econstructor; [rewrite <- HRApp1 | rewrite <- HRApp2]; constructor.
   Case "cond_true".  
     edestruct IHD1 as [sttyb [Weakb [TcHeapvb TcVal_e0]]]; eauto. 
@@ -651,6 +670,8 @@ Proof.
        simpl in H; inversion H; subst. 
        rewrite subst_rho_tyref. unfold mk_rgn_type. rewrite subst_rho_rgn_const.
        econstructor. apply ST_same_key_1.
+       intro.
+       eapply TcVal_implies_closed in TcVal_v; eauto.
   Case "get_ref e".    
     destruct IHD with (hp'0 := hp')
                       (v := Loc (Rgn2_Const true false s) l) 
